define swap partl second

example_array.v
@@ -2,7 +2,7 @@
 (* Copyright (C) 2020 monae authors, license: LGPL-2.1-or-later               *)
 From mathcomp Require Import all_ssreflect.
 From mathcomp Require boolp.
-Require Import monae_lib hierarchy monad_lib fail_lib state_lib.
+Require Import monae_lib hierarchy monad_lib fail_lib state_lib example_quicksort.
 From infotheo Require Import ssr_ext.
 
 (*******************************************************************************)
@@ -23,6 +23,7 @@ Require Import ZArith.
 
 Section marray.
 Variables (E : UU0) (M : arrayMonad E Z_eqType).
+Variables (d : unit) (T : porderType d).
 
 Fixpoint readList (i : Z) (n : nat) : M (seq E) :=
   if n isn't k.+1 then Ret [::] else liftM2 cons (aget i) (readList (i + 1) k).
@@ -35,8 +36,31 @@ Definition writeL (i : Z) (s : seq E) := writeList i s >> Ret (size s).
 Definition write2L (i : Z) '(s1, s2) :=
   writeList i (s1 ++ s2) >> Ret (size s1, size s2).
 
-Definition write3L i '(xs, ys, zs) :=
+Definition write3L (i : Z) '(xs, ys, zs) :=
   writeList i (xs ++ ys ++ zs) >> Ret (size xs, size ys, size zs).
+
+Definition swap (i j : Z) : M unit := 
+  aGet i >>= (fun x => aGet j >>= (fun y => aPut i y >> aPut j x)).
+
+Fixpoint partl (p : T) (s : (seq T * seq T)%type) (xs : seq T): (seq T * seq T)%type :=
+  match xs with
+  | [::] => s
+  | x :: xs => if x <= p then partl p (s.1 ++ [:: x], s.2) xs
+                                   else partl p (s.1, s.2 ++ [:: x]) xs
+  end.
+
+Definition second {A B C} (f : B -> M C) (xy : (A * B)%type) := f xy.2 >>= (fun y' => Ret (xy.1, y')).
+
+Program Fixpoint partl' (p : T) (s : (seq T * seq T)) (xs : seq T): M (seq T * seq T)%type :=
+  match xs with
+  | [::] => Ret s
+  | x :: xs => if x <= p then qperm s.2 >>= (fun zs' => partl' p (s.1 ++ [:: x], s.2) xs)
+                         else partl' p (s.1, s.2 ++ [:: x]) xs
+  end.
+
+Lemma ipartl_spec (i : Z) (p : E) (ys zs xs : seq E) (ipartl : E -> Z -> (nat * nat * nat)%type -> M (nat * nat)%type): 
+  writeList i (ys ++ zs ++ xs) >> ipartl p i (size ys, size zs, size xs)
+    `<=` second perm (partl p (ys, zs) xs) >>= write2L i.
 
 Local Open Scope zarith_ext_scope.
 
